\documentclass{article}
\usepackage{jheppub,physics,amsfonts,graphicx,tensor,cleveref}
\usepackage[export]{adjustbox}
\newcommand{\ii}{\mathrm{i}}
\newcommand{\me}{\mathrm{e}}
\newcommand{\cd}{\mathcal{D}}
\DeclareMathOperator{\arcsinh}{arcsinh}
\DeclareMathOperator{\sgn}{sgn}
\counterwithout{equation}{section}


\title{Homework 4}
\author{Shangjie Zhou}
\emailAdd{zhou1468@purdue.edu}
\toccontinuoustrue
\notoc


\begin{document}

\maketitle


\section*{Problem 1}
\subsection*{(a)}
\subsubsection*{(i)}
From the commutation relation of the angular momentum operators, we have
\begin{subequations}
    \begin{align}
        S_z S_x-S_x S_z&=\ii \hbar S_y,\\
        S_y S_z-S_z S_y&=\ii \hbar S_x,
    \end{align}
\end{subequations}
which gives
\begin{subequations}
    \begin{align}
        \bra{S,S}(S_z S_x-S_x S_z)\ket{S,S}&=\ii \hbar \bra{S,S}S_y\ket{S,S},\\
        \bra{S,S}(S_y S_z-S_z S_y)\ket{S,S}&=\ii \hbar \bra{S,S}S_x\ket{S,S}.
    \end{align}
\end{subequations}
Since $S_z\ket{S,S}=\hbar S\ket{S,S}$, we have
\begin{subequations}
    \begin{align}
        \bra{S,S}(S_z S_x-S_x S_z)\ket{S,S}&=\hbar S \bra{S,S}S_x\ket{S,S}-\hbar S \bra{S,S}S_x\ket{S,S}=0,\\
        \bra{S,S}(S_y S_z-S_z S_y)\ket{S,S}&=\hbar S \bra{S,S}S_y\ket{S,S}-\hbar S \bra{S,S}S_y\ket{S,S}=0.
    \end{align}
    \end{subequations}
Thus, we have
\begin{subequations}
    \begin{align}
        \bra{S,S}S_y\ket{S,S}&=0,\\
        \bra{S,S}S_x\ket{S,S}&=0.
    \end{align}
\end{subequations}
\subsubsection*{(ii)}
Since $U=\exp(-\ii \phi S_z/\hbar)\exp(\ii \theta S_y/\hbar)$, we can use Baker–Campbell–Hausdorff formula and compute that
\begin{equation}
    U^\dagger S_z U=\exp(-\ii \theta S_y/\hbar)\,S_z\,\exp(\ii \theta S_y/\hbar).
\end{equation}
To evaluate this we set
\[A=\ii\frac{\theta}{\hbar}S_y,\qquad\text{so}\qquad U^\dagger S_z U=e^{-A}S_z e^{A},\]
and use the Baker--Campbell--Hausdorff (conjugation) expansion
\[e^{-A}S_z e^{A}=S_z+[S_z,A]+\frac{1}{2!}[[S_z,A],A]+\frac{1}{3!}[[[S_z,A],A],A]+\cdots.\]
Compute the first commutators using $[S_i,S_j]=\ii\hbar\epsilon_{ijk}S_k$:
\begin{align*}
    [S_z,A]&=\ii\frac{\theta}{\hbar}[S_z,S_y]=\ii\frac{\theta}{\hbar}(-\ii\hbar S_x)=\theta S_x,\\
    [[S_z,A],A]&=\theta[S_x,A]=\theta\left(\ii\frac{\theta}{\hbar}[S_x,S_y]\right)=\theta\left(\ii\frac{\theta}{\hbar}(\ii\hbar S_z)\right)=-\theta^2 S_z.
\end{align*}
Substituting into the series gives
\begin{align*}
    e^{-A}S_z e^{A}&=S_z+\theta S_x-\frac{\theta^2}{2!}S_z-\frac{\theta^3}{3!}S_x+\frac{\theta^4}{4!}S_z+\cdots\\
    &=S_z\Big(1-\frac{\theta^2}{2!}+\frac{\theta^4}{4!}-\cdots\Big)+S_x\Big(\theta-\frac{\theta^3}{3!}+\frac{\theta^5}{5!}-\cdots\Big)\\
    &=S_z\cos\theta+S_x\sin\theta.
\end{align*}


%\bibliographystyle{jhep}
%\bibliography{ref}
\end{document}